Source/DafnyRuntime/DafnyRuntimeJava/src/main/generated-java/Dafny/ArraySequence.java
@@ -1,0 +1,59 @@
+// Class ArraySequence
+// Dafny class ArraySequence compiled into Java
+package Dafny;
+
+
+@SuppressWarnings({"unchecked", "deprecation"})
+public class ArraySequence<T> implements Sequence<T> {
+  private dafny.TypeDescriptor<T> _td_T;
+  public ArraySequence(dafny.TypeDescriptor<T> _td_T) {
+    this._td_T = _td_T;
+    this._value = null;
+  }
+  public T Select(java.math.BigInteger index)
+  {
+    @SuppressWarnings({"unchecked", "deprecation"})
+    T _out9;
+    _out9 = Dafny._Companion_Sequence.<T>Select(_td_T, this, index);
+    return _out9;
+  }
+  public Sequence<T> Drop(java.math.BigInteger lo)
+  {
+    Sequence<T> _out10;
+    _out10 = Dafny._Companion_Sequence.<T>Drop(_td_T, this, lo);
+    return _out10;
+  }
+  public Sequence<T> Take(java.math.BigInteger hi)
+  {
+    Sequence<T> _out11;
+    _out11 = Dafny._Companion_Sequence.<T>Take(_td_T, this, hi);
+    return _out11;
+  }
+  public Sequence<T> Subsequence(java.math.BigInteger lo, java.math.BigInteger hi)
+  {
+    Sequence<T> _out12;
+    _out12 = Dafny._Companion_Sequence.<T>Subsequence(_td_T, this, lo, hi);
+    return _out12;
+  }
+  public void __ctor(ImmutableArray<T> value)
+  {
+    (this)._value = value;
+  }
+  public java.math.BigInteger Length() {
+    return ((this).value()).Length();
+  }
+  public ImmutableArray<T> ToArray()
+  {
+    ImmutableArray<T> ret = null;
+    ret = (this).value();
+    return ret;
+  }
+  public ImmutableArray<T> _value;
+  public ImmutableArray<T> value()
+  {
+    return this._value;
+  }
+  public static <T> dafny.TypeDescriptor<ArraySequence<T>> _typeDescriptor(dafny.TypeDescriptor<T> _td_T) {
+    return (dafny.TypeDescriptor<ArraySequence<T>>) (dafny.TypeDescriptor<?>) dafny.TypeDescriptor.referenceWithInitializer(ArraySequence.class, () -> (ArraySequence<T>) null);
+  }
+}
