Source/DafnyRuntime/DafnyRuntimeJava/src/main/generated-java/Dafny/Sequence.java
@@ -1,0 +1,14 @@
+// Interface Sequence
+// Dafny trait Sequence compiled into Java
+package Dafny;
+
+
+@SuppressWarnings({"unchecked", "deprecation"})
+public interface Sequence<T> {
+  public java.math.BigInteger Length();
+  public T Select(java.math.BigInteger index);
+  public Sequence<T> Drop(java.math.BigInteger lo);
+  public Sequence<T> Take(java.math.BigInteger hi);
+  public Sequence<T> Subsequence(java.math.BigInteger lo, java.math.BigInteger hi);
+  public ImmutableArray<T> ToArray();
+}
