Source/DafnyRuntime/DafnyRuntimeJava/src/main/generated-java/Dafny/_ExternBase___default.java
@@ -1,0 +1,103 @@
+// Class _ExternBase___default
+// Dafny class __default compiled into Java
+package Dafny;
+
+
+@SuppressWarnings({"unchecked", "deprecation"})
+public abstract class _ExternBase___default {
+  public _ExternBase___default() {
+  }
+  public static <__T> Sequence<__T> Concatenate(dafny.TypeDescriptor<__T> _td___T, Sequence<__T> left, Sequence<__T> right)
+  {
+    Sequence<__T> ret = null;
+    if(true) {
+      ConcatSequence<__T> _12_c;
+      ConcatSequence<__T> _nw4 = new ConcatSequence<__T>(_td___T);
+      _nw4.__ctor(left, right);
+      _12_c = _nw4;
+      LazySequence<__T> _nw5 = new LazySequence<__T>(_td___T);
+      _nw5.__ctor(_12_c);
+      ret = _nw5;
+    }
+    return ret;
+  }
+  public static <__T> void AppendRecursive(dafny.TypeDescriptor<__T> _td___T, Vector<__T> builder, Sequence<__T> e)
+  {
+    if (dafny.Helpers.<Sequence<__T>, Boolean>Let(e, _is_0 -> _is_0 instanceof ConcatSequence)) {
+      ConcatSequence<__T> _13_concat;
+      _13_concat = ((ConcatSequence<__T>)(e));
+      __default.<__T>AppendRecursive(_td___T, builder, (_13_concat).left());
+      __default.<__T>AppendRecursive(_td___T, builder, (_13_concat).right());
+    } else if (dafny.Helpers.<Sequence<__T>, Boolean>Let(e, _is_1 -> _is_1 instanceof LazySequence)) {
+      LazySequence<__T> _14_lazy;
+      _14_lazy = ((LazySequence<__T>)(e));
+      Sequence<__T> _15_boxed;
+      Sequence<__T> _out25;
+      _out25 = ((_14_lazy).box()).Get();
+      _15_boxed = _out25;
+      __default.<__T>AppendRecursive(_td___T, builder, _15_boxed);
+    } else {
+      ImmutableArray<__T> _16_a;
+      ImmutableArray<__T> _out26;
+      _out26 = (e).ToArray();
+      _16_a = _out26;
+      (builder).Append(_16_a);
+    }
+  }
+  public static <__T> void AppendOptimized(dafny.TypeDescriptor<__T> _td___T, Vector<__T> builder, Sequence<__T> e, Vector<Sequence<__T>> stack)
+  {
+    TAIL_CALL_START: while (true) {
+      if(true) {
+        if (dafny.Helpers.<Sequence<__T>, Boolean>Let(e, _is_2 -> _is_2 instanceof ConcatSequence)) {
+          ConcatSequence<__T> _17_concat;
+          _17_concat = ((ConcatSequence<__T>)(e));
+          (stack).AddLast((_17_concat).right());
+          Vector<__T> _in0 = builder;
+          Sequence<__T> _in1 = (_17_concat).left();
+          Vector<Sequence<__T>> _in2 = stack;
+          builder = _in0;
+          e = _in1;
+          stack = _in2;
+          continue TAIL_CALL_START;
+        } else if (dafny.Helpers.<Sequence<__T>, Boolean>Let(e, _is_3 -> _is_3 instanceof LazySequence)) {
+          LazySequence<__T> _18_lazy;
+          _18_lazy = ((LazySequence<__T>)(e));
+          Sequence<__T> _19_boxed;
+          Sequence<__T> _out27;
+          _out27 = ((_18_lazy).box()).Get();
+          _19_boxed = _out27;
+          Vector<__T> _in3 = builder;
+          Sequence<__T> _in4 = _19_boxed;
+          Vector<Sequence<__T>> _in5 = stack;
+          builder = _in3;
+          e = _in4;
+          stack = _in5;
+          continue TAIL_CALL_START;
+        } else if (dafny.Helpers.<Sequence<__T>, Boolean>Let(e, _is_4 -> _is_4 instanceof ArraySequence)) {
+          ArraySequence<__T> _20_a;
+          _20_a = ((ArraySequence<__T>)(e));
+          (builder).Append((_20_a).value());
+          if ((stack.size).signum() == 1) {
+            Sequence<__T> _21_next;
+            Sequence<__T> _out28;
+            _out28 = (stack).RemoveLast();
+            _21_next = _out28;
+            Vector<__T> _in6 = builder;
+            Sequence<__T> _in7 = _21_next;
+            Vector<Sequence<__T>> _in8 = stack;
+            builder = _in6;
+            e = _in7;
+            stack = _in8;
+            continue TAIL_CALL_START;
+          }
+        } else {
+        }
+      }
+      return;
+    }
+  }
+  private static final dafny.TypeDescriptor<__default> _TYPE = dafny.TypeDescriptor.referenceWithInitializer(__default.class, () -> (__default) null);
+  public static dafny.TypeDescriptor<__default> _typeDescriptor() {
+    return (dafny.TypeDescriptor<__default>) (dafny.TypeDescriptor<?>) _TYPE;
+  }
+}
