Source/DafnyRuntime/generated.cs
@@ -1,4 +1,4 @@
-// Dafny program array.dfy compiled into C#
+// Dafny program dafnyRuntime.dfy compiled into C#
 // To recompile, you will need the libraries
 //     System.Runtime.Numerics.dll System.Collections.Immutable.dll
 // but the 'dotnet' tool in net6.0 should pick those up automatically.
@@ -9,14 +9,40 @@ using System;
 using System.Numerics;
 using System.Collections;
 [assembly: DafnyAssembly.DafnySourceAttribute(@"// Dafny 3.7.2.40713
-// Command Line Options: /noVerify /compile:0 /spillTargetCode:3 /useRuntimeLib src/array.dfy /compileTarget:cs /out:../DafnyRuntime/generated
-// array.dfy
+// Command Line Options: /noVerify /compile:0 /spillTargetCode:3 /useRuntimeLib src/dafnyRuntime.dfy /compileTarget:cs /out:../DafnyRuntime/generated
+// dafnyRuntime.dfy
 
 
-module {:extern ""Arrays""} {:options ""/functionSyntax:4""} Arrays {
+module {:extern ""Dafny""} {:options ""/functionSyntax:4""} Dafny {
+  trait Validatable {
+    ghost var Repr: set<object>
 
-  import opened Frames
-  trait {:extern} {:termination false} Array<T> extends Validatable {
+    predicate Valid()
+      reads this, Repr
+      ensures Valid() ==> this in Repr
+      decreases Repr, 1
+
+    predicate ValidComponent(component: Validatable)
+      reads this, Repr
+      decreases Repr, 0
+    {
+      this in Repr &&
+      component in Repr &&
+      component.Repr <= Repr &&
+      this !in component.Repr &&
+      assert component.Repr < Repr; component.Valid()
+    }
+
+    twostate predicate ValidAndDisjoint()
+      reads this, Repr
+      decreases Repr + {this}
+    {
+      Valid() &&
+      fresh(Repr - old(Repr))
+    }
+  }
+
+  trait {:extern} Array<T> extends Validatable {
     ghost var values: seq<ArrayCell<T>>
 
     function method Length(): nat
@@ -66,7 +92,7 @@ module {:extern ""Arrays""} {:options ""/functionSyntax:4""} Arrays {
 
   datatype ArrayCell<T> = Set(value: T) | Unset
 
-  trait {:extern} {:termination false} ImmutableArray<+T> {
+  trait {:extern} ImmutableArray<+T> {
     ghost const values: seq<T>
 
     predicate Valid()
@@ -103,10 +129,13 @@ module {:extern ""Arrays""} {:options ""/functionSyntax:4""} Arrays {
     predicate Valid()
       reads this, Repr
       ensures Valid() ==> this in Repr
-      decreases Repr + {this}
+      decreases Repr, 1
     {
       this in Repr &&
-      ValidComponent(storage) &&
+      storage in Repr &&
+      storage.Repr <= Repr &&
+      this !in storage.Repr &&
+      storage.Valid() &&
       0 <= size <= storage.Length() &&
       forall i: int | 0 <= i < size :: 
         storage.values[i].Set?
@@ -228,50 +257,353 @@ module {:extern ""Arrays""} {:options ""/functionSyntax:4""} Arrays {
     }
   }
 
+  class {:extern} AtomicBox<!T> {
+    ghost const inv: T -> bool
+
+    static method {:extern} Make(ghost inv: T -> bool, t: T) returns (ret: AtomicBox<T>)
+      requires inv(t)
+      ensures ret.inv == inv
+
+    method {:extern} Get() returns (t: T)
+      ensures inv(t)
+
+    method {:extern} Put(t: T)
+      requires inv(t)
+  }
+
+  trait {:extern} Sequence<+T> {
+    ghost const size: nat
+
+    predicate Valid()
+      ensures Valid() ==> 0 < size
+      decreases size, 0
+
+    function method Length(): nat
+      requires Valid()
+      decreases size, 1
+
+    function Value(): seq<T>
+      requires Valid()
+      ensures |Value()| == Length()
+      decreases size, 2
+
+    method Select(index: nat) returns (ret: T)
+      requires Valid()
+      requires index < Length()
+      ensures ret == Value()[index]
+      decreases index
+    {
+      var a := ToArray();
+      return a.At(index);
+    }
+
+    method Drop(lo: nat) returns (ret: Sequence<T>)
+      requires Valid()
+      requires lo <= Length()
+      ensures ret.Valid()
+      ensures ret.Value() == Value()[lo..]
+      decreases size, 2
+    {
+      ret := Subsequence(lo, Length());
+    }
+
+    method Take(hi: nat) returns (ret: Sequence<T>)
+      requires Valid()
+      requires hi <= Length()
+      ensures ret.Valid()
+      ensures ret.Value() == Value()[..hi]
+      decreases size, 2
+    {
+      ret := Subsequence(0, hi);
+    }
+
+    method Subsequence(lo: nat, hi: nat) returns (ret: Sequence<T>)
+      requires Valid()
+      requires lo <= hi <= Length()
+      ensures ret.Valid()
+      ensures ret.Value() == Value()[lo .. hi]
+      decreases size, 2
+    {
+      var a := ToArray();
+      var subarray := a.Subarray(lo, hi);
+      ret := new ArraySequence<T>(subarray);
+    }
+
+    method ToArray() returns (ret: ImmutableArray<T>)
+      requires Valid()
+      ensures ret.Valid()
+      ensures ret.Length() == Length()
+      ensures ret.values == Value()
+      decreases size, 2
+  }
+
+  class ArraySequence<T> extends Sequence<T> {
+    const value: ImmutableArray<T>
+
+    predicate Valid()
+      ensures Valid() ==> 0 < size
+      decreases size, 0
+    {
+      value.Valid() &&
+      size == 1
+    }
+
+    constructor (value: ImmutableArray<T>)
+      requires value.Valid()
+      ensures Valid()
+      ensures this.value == value
+      decreases value
+    {
+      this.value := value;
+      this.size := 1;
+    }
+
+    function method Length(): nat
+      requires Valid()
+      decreases size, 1
+    {
+      value.Length()
+    }
+
+    function Value(): seq<T>
+      requires Valid()
+      ensures |Value()| == Length()
+      decreases size, 2
+    {
+      value.values
+    }
+
+    method ToArray() returns (ret: ImmutableArray<T>)
+      requires Valid()
+      ensures ret.Valid()
+      ensures ret.Length() == Length()
+      ensures ret.values == Value()
+      decreases size, 2
+    {
+      return value;
+    }
+  }
+
+  class ConcatSequence<T> extends Sequence<T> {
+    const left: Sequence<T>
+    const right: Sequence<T>
+    const length: nat
+
+    predicate Valid()
+      ensures Valid() ==> 0 < size
+      decreases size, 0
+    {
+      size == 1 + left.size + right.size &&
+      left.Valid() &&
+      right.Valid() &&
+      length == left.Length() + right.Length()
+    }
+
+    constructor (left: Sequence<T>, right: Sequence<T>)
+      requires left.Valid()
+      requires right.Valid()
+      ensures Valid()
+      decreases left, right
+    {
+      this.left := left;
+      this.right := right;
+      this.length := left.Length() + right.Length();
+      this.size := 1 + left.size + right.size;
+    }
+
+    function method Length(): nat
+      requires Valid()
+      decreases size, 1
+    {
+      length
+    }
+
+    function Value(): seq<T>
+      requires Valid()
+      ensures |Value()| == Length()
+      decreases size, 2
+    {
+      ghost var ret: seq<T> := left.Value() + right.Value();
+      assert |ret| == Length();
+      ret
+    }
+
+    method ToArray() returns (ret: ImmutableArray<T>)
+      requires Valid()
+      ensures ret.Valid()
+      ensures ret.Length() == Length()
+      ensures ret.values == Value()
+      decreases size, 2
+    {
+      var builder := new Vector<T>(length);
+      var stack := new Vector<Sequence<T>>(10);
+      AppendOptimized(builder, this, stack);
+      ret := builder.Freeze();
+    }
+  }
+
+  class LazySequence<T> extends Sequence<T> {
+    ghost const value: seq<T>
+    const box: AtomicBox<Sequence<T>>
+    const length: nat
+
+    predicate Valid()
+      ensures Valid() ==> 0 < size
+      decreases size, 0
+    {
+      0 < size &&
+      length == |value| &&
+      box.inv == (s: Sequence<T>) => s.size < size && s.Valid() && s.Value() == value
+    }
+
+    predicate Call(s: Sequence<T>)
+      decreases s
+    {
+      s.size < size &&
+      s.Valid() &&
+      s.Value() == value
+    }
+
+    constructor (wrapped: Sequence<T>)
+      requires wrapped.Valid()
+      requires 1 <= wrapped.size
+      ensures Valid()
+      decreases wrapped
+    {
+      ghost var value := wrapped.Value();
+      ghost var size := 1 + wrapped.size;
+      ghost var inv := (s: Sequence<T>) => s.size < size && s.Valid() && s.Value() == value;
+      var box := AtomicBox.Make(inv, wrapped);
+      this.box := box;
+      this.length := wrapped.Length();
+      this.value := value;
+      this.size := size;
+    }
+
+    function method Length(): nat
+      requires Valid()
+      decreases size, 1
+    {
+      length
+    }
+
+    function Value(): seq<T>
+      requires Valid()
+      ensures |Value()| == Length()
+      decreases size, 2
+    {
+      assert |value| == Length();
+      value
+    }
+
+    method ToArray() returns (ret: ImmutableArray<T>)
+      requires Valid()
+      ensures ret.Valid()
+      ensures ret.Length() == Length()
+      ensures ret.values == Value()
+      decreases size, 2
+    {
+      var expr := box.Get();
+      ret := expr.ToArray();
+      var arraySeq := new ArraySequence<T>(ret);
+      box.Put(arraySeq);
+    }
+  }
+
   method {:extern} NewArray<T>(length: nat) returns (ret: Array<T>)
     ensures ret.Valid()
     ensures fresh(ret.Repr)
     ensures ret.Length() == length
     decreases length
-}
 
-module {:options ""/functionSyntax:4""} Frames {
-  trait {:termination false} Validatable {
-    ghost var Repr: set<object>
+  lemma {:axiom} SequenceTypeIsClosed<T>(e: Sequence<T>)
+    ensures e is ArraySequence<T> || e is ConcatSequence<T> || e is LazySequence<T>
+    decreases e
 
-    predicate Valid()
-      reads this, Repr
-      ensures Valid() ==> this in Repr
-      decreases Repr + {this}
+  method Concatenate<T>(left: Sequence<T>, right: Sequence<T>) returns (ret: Sequence<T>)
+    requires left.Valid()
+    requires right.Valid()
+    ensures ret.Valid()
+    decreases left, right
+  {
+    var c := new ConcatSequence<T>(left, right);
+    ret := new LazySequence<T>(c);
+  }
 
-    predicate ValidComponent(component: Validatable)
-      reads this, Repr
-      decreases Repr + {this}, component
-    {
-      component in Repr &&
-      component.Repr <= Repr &&
-      this !in component.Repr &&
-      component.Valid()
-    }
-
-    twostate predicate ValidAndDisjoint()
-      reads this, Repr
-      decreases Repr + {this}
-    {
-      Valid() &&
-      fresh(Repr - old(Repr))
+  method AppendRecursive<T>(builder: Vector<T>, e: Sequence<T>)
+    requires e.Valid()
+    requires builder.Valid()
+    modifies builder.Repr
+    ensures builder.ValidAndDisjoint()
+    ensures e.Valid()
+    ensures builder.Value() == old(builder.Value()) + e.Value()
+    decreases e.size
+  {
+    if e is ConcatSequence<T> {
+      var concat := e as ConcatSequence<T>;
+      AppendRecursive(builder, concat.left);
+      AppendRecursive(builder, concat.right);
+    } else if e is LazySequence<T> {
+      var lazy := e as LazySequence<T>;
+      var boxed := lazy.box.Get();
+      AppendRecursive(builder, boxed);
+    } else {
+      var a: ImmutableArray<T> := e.ToArray();
+      builder.Append(a);
     }
   }
 
-  predicate PairwiseDisjoint(s: set<Validatable>)
-    reads s, set v: Validatable, o: object {:trigger o in v.Repr} | v in s && o in v.Repr :: o
-    decreases s + set v: Validatable, o: object {:trigger o in v.Repr} | v in s && o in v.Repr :: o, s
+  method {:tailrecursion} AppendOptimized<T>(builder: Vector<T>, e: Sequence<T>, stack: Vector<Sequence<T>>)
+    requires e.Valid()
+    requires builder.Valid()
+    requires stack.Valid()
+    requires builder.Repr !! stack.Repr
+    requires forall expr: Sequence<T> | expr in stack.Value() :: expr.Valid()
+    modifies builder.Repr, stack.Repr
+    ensures builder.Valid()
+    ensures stack.Valid()
+    ensures builder.Value() == old(builder.Value()) + e.Value() + ConcatValueOnStack(old(stack.Value()))
+    decreases e.size + SizeSum(stack.Value())
   {
-    true &&
-    forall v: Validatable | v in s :: 
-      v.Valid() &&
-      forall v: Validatable, v': Validatable | v in s && v' in s && v != v' :: 
-        v.Repr !! v'.Repr
+    if e is ConcatSequence<T> {
+      var concat := e as ConcatSequence<T>;
+      stack.AddLast(concat.right);
+      AppendOptimized(builder, concat.left, stack);
+    } else if e is LazySequence<T> {
+      var lazy := e as LazySequence<T>;
+      var boxed := lazy.box.Get();
+      AppendOptimized(builder, boxed, stack);
+    } else if e is ArraySequence<T> {
+      var a := e as ArraySequence<T>;
+      builder.Append(a.value);
+      if 0 < stack.size {
+        var next: Sequence<T> := stack.RemoveLast();
+        AppendOptimized(builder, next, stack);
+      }
+    } else {
+      SequenceTypeIsClosed(e);
+      assert false;
+    }
+  }
+
+  function ConcatValueOnStack<T>(s: seq<Sequence<T>>): seq<T>
+    requires forall e: Sequence<T> | e in s :: e.Valid()
+    decreases s
+  {
+    if |s| == 0 then
+      []
+    else
+      s[|s| - 1].Value() + ConcatValueOnStack(s[..|s| - 1])
+  }
+
+  function SizeSum<T>(s: seq<Sequence<T>>): nat
+    requires forall e: Sequence<T> | e in s :: e.Valid()
+    decreases s
+  {
+    if |s| == 0 then
+      0
+    else
+      ghost var last: int := |s| - 1; SizeSum(s[..last]) + s[last].size
   }
 }
 ")]
@@ -308,22 +640,19 @@ namespace _System {
     }
   }
 } // end of namespace _System
-namespace Frames_Compile {
+namespace Dafny {
 
   public interface Validatable {
   }
   public class _Companion_Validatable {
   }
 
-} // end of namespace Frames_Compile
-namespace Arrays {
-
-  public interface Array<T> : Frames_Compile.Validatable {
+  public interface Array<T> : Dafny.Validatable {
     BigInteger Length();
     T Read(BigInteger i);
     void Write(BigInteger i, T t);
-    void WriteRangeArray(BigInteger start, Arrays.ImmutableArray<T> other);
-    Arrays.ImmutableArray<T> Freeze(BigInteger size);
+    void WriteRangeArray(BigInteger start, Dafny.ImmutableArray<T> other);
+    Dafny.ImmutableArray<T> Freeze(BigInteger size);
   }
   public class _Companion_Array<T> {
   }
@@ -339,8 +668,8 @@ namespace Arrays {
     public static _IArrayCell<T> Default() {
       return create_Unset();
     }
-    public static Dafny.TypeDescriptor<Arrays._IArrayCell<T>> _TypeDescriptor() {
-      return new Dafny.TypeDescriptor<Arrays._IArrayCell<T>>(Arrays.ArrayCell<T>.Default());
+    public static Dafny.TypeDescriptor<Dafny._IArrayCell<T>> _TypeDescriptor() {
+      return new Dafny.TypeDescriptor<Dafny._IArrayCell<T>>(Dafny.ArrayCell<T>.Default());
     }
     public static _IArrayCell<T> create_Set(T @value) {
       return new ArrayCell_Set<T>(@value);
@@ -368,7 +697,7 @@ namespace Arrays {
       return new ArrayCell_Set<__T>(converter0(@value));
     }
     public override bool Equals(object other) {
-      var oth = other as Arrays.ArrayCell_Set<T>;
+      var oth = other as Dafny.ArrayCell_Set<T>;
       return oth != null && object.Equals(this.@value, oth.@value);
     }
     public override int GetHashCode() {
@@ -378,7 +707,7 @@ namespace Arrays {
       return (int) hash;
     }
     public override string ToString() {
-      string s = "Arrays_Compile.ArrayCell.Set";
+      string s = "Dafny_Compile.ArrayCell.Set";
       s += "(";
       s += Dafny.Helpers.ToString(this.@value);
       s += ")";
@@ -393,7 +722,7 @@ namespace Arrays {
       return new ArrayCell_Unset<__T>();
     }
     public override bool Equals(object other) {
-      var oth = other as Arrays.ArrayCell_Unset<T>;
+      var oth = other as Dafny.ArrayCell_Unset<T>;
       return oth != null;
     }
     public override int GetHashCode() {
@@ -402,7 +731,7 @@ namespace Arrays {
       return (int) hash;
     }
     public override string ToString() {
-      string s = "Arrays_Compile.ArrayCell.Unset";
+      string s = "Dafny_Compile.ArrayCell.Unset";
       return s;
     }
   }
@@ -410,23 +739,23 @@ namespace Arrays {
   public interface ImmutableArray<out T> {
     BigInteger Length();
     T At(BigInteger index);
-    Arrays.ImmutableArray<T> Subarray(BigInteger lo, BigInteger hi);
+    Dafny.ImmutableArray<T> Subarray(BigInteger lo, BigInteger hi);
   }
   public class _Companion_ImmutableArray<T> {
   }
 
-  public partial class Vector<T> : Frames_Compile.Validatable {
+  public partial class Vector<T> : Dafny.Validatable {
     public Vector() {
-      this.storage = default(Arrays.Array<T>);
+      this.storage = default(Dafny.Array<T>);
       this.size = BigInteger.Zero;
     }
-    public  Arrays.Array<T> storage {get; set;}
+    public  Dafny.Array<T> storage {get; set;}
     public  BigInteger size {get; set;}
     public void __ctor(BigInteger length)
     {
-      Arrays.Array<T> _0_storage;
-      Arrays.Array<T> _out0;
-      _out0 = Arrays.__default.NewArray<T>(length);
+      Dafny.Array<T> _0_storage;
+      Dafny.Array<T> _out0;
+      _out0 = Dafny.__default.NewArray<T>(length);
       _0_storage = _out0;
       (this).storage = _0_storage;
       (this).size = BigInteger.Zero;
@@ -455,12 +784,12 @@ namespace Arrays {
     }
     public void Reallocate(BigInteger newCapacity)
     {
-      Arrays.Array<T> _1_newStorage;
-      Arrays.Array<T> _out1;
-      _out1 = Arrays.__default.NewArray<T>(newCapacity);
+      Dafny.Array<T> _1_newStorage;
+      Dafny.Array<T> _out1;
+      _out1 = Dafny.__default.NewArray<T>(newCapacity);
       _1_newStorage = _out1;
-      Arrays.ImmutableArray<T> _2_values;
-      Arrays.ImmutableArray<T> _out2;
+      Dafny.ImmutableArray<T> _2_values;
+      Dafny.ImmutableArray<T> _out2;
       _out2 = (this.storage).Freeze(this.size);
       _2_values = _out2;
       (_1_newStorage).WriteRangeArray(BigInteger.Zero, _2_values);
@@ -473,7 +802,7 @@ namespace Arrays {
       (this).size = (this.size) - (BigInteger.One);
       return t;
     }
-    public void Append(Arrays.ImmutableArray<T> other)
+    public void Append(Dafny.ImmutableArray<T> other)
     {
       BigInteger _3_newSize;
       _3_newSize = (this.size) + ((other).Length());
@@ -483,10 +812,10 @@ namespace Arrays {
       (this.storage).WriteRangeArray(this.size, other);
       (this).size = (this.size) + ((other).Length());
     }
-    public Arrays.ImmutableArray<T> Freeze()
+    public Dafny.ImmutableArray<T> Freeze()
     {
-      Arrays.ImmutableArray<T> ret = default(Arrays.ImmutableArray<T>);
-      Arrays.ImmutableArray<T> _out3;
+      Dafny.ImmutableArray<T> ret = default(Dafny.ImmutableArray<T>);
+      Dafny.ImmutableArray<T> _out3;
       _out3 = (this.storage).Freeze(this.size);
       ret = _out3;
       return ret;
@@ -496,7 +825,333 @@ namespace Arrays {
     } }
   }
 
-} // end of namespace Arrays
+
+  public interface Sequence<out T> {
+    BigInteger Length();
+    T Select(BigInteger index);
+    Dafny.Sequence<T> Drop(BigInteger lo);
+    Dafny.Sequence<T> Take(BigInteger hi);
+    Dafny.Sequence<T> Subsequence(BigInteger lo, BigInteger hi);
+    Dafny.ImmutableArray<T> ToArray();
+  }
+  public class _Companion_Sequence<T> {
+    public static T Select(Dafny.Sequence<T> _this, BigInteger index)
+    {
+      T ret = default(T);
+      Dafny.ImmutableArray<T> _4_a;
+      Dafny.ImmutableArray<T> _out4;
+      _out4 = (_this).ToArray();
+      _4_a = _out4;
+      ret = (_4_a).At(index);
+      return ret;
+      return ret;
+    }
+    public static Dafny.Sequence<T> Drop(Dafny.Sequence<T> _this, BigInteger lo)
+    {
+      Dafny.Sequence<T> ret = default(Dafny.Sequence<T>);
+      Dafny.Sequence<T> _out5;
+      _out5 = (_this).Subsequence(lo, (_this).Length());
+      ret = _out5;
+      return ret;
+    }
+    public static Dafny.Sequence<T> Take(Dafny.Sequence<T> _this, BigInteger hi)
+    {
+      Dafny.Sequence<T> ret = default(Dafny.Sequence<T>);
+      Dafny.Sequence<T> _out6;
+      _out6 = (_this).Subsequence(BigInteger.Zero, hi);
+      ret = _out6;
+      return ret;
+    }
+    public static Dafny.Sequence<T> Subsequence(Dafny.Sequence<T> _this, BigInteger lo, BigInteger hi)
+    {
+      Dafny.Sequence<T> ret = default(Dafny.Sequence<T>);
+      Dafny.ImmutableArray<T> _5_a;
+      Dafny.ImmutableArray<T> _out7;
+      _out7 = (_this).ToArray();
+      _5_a = _out7;
+      Dafny.ImmutableArray<T> _6_subarray;
+      Dafny.ImmutableArray<T> _out8;
+      _out8 = (_5_a).Subarray(lo, hi);
+      _6_subarray = _out8;
+      Dafny.ArraySequence<T> _nw0 = new Dafny.ArraySequence<T>();
+      _nw0.__ctor(_6_subarray);
+      ret = _nw0;
+      return ret;
+    }
+  }
+
+  public partial class ArraySequence<T> : Dafny.Sequence<T> {
+    public ArraySequence() {
+      this._value = default(Dafny.ImmutableArray<T>);
+    }
+    public T Select(BigInteger index)
+    {
+      T _out9;
+      _out9 = Dafny._Companion_Sequence<T>.Select(this, index);
+      return _out9;
+    }
+    public Dafny.Sequence<T> Drop(BigInteger lo)
+    {
+      Dafny.Sequence<T> _out10;
+      _out10 = Dafny._Companion_Sequence<T>.Drop(this, lo);
+      return _out10;
+    }
+    public Dafny.Sequence<T> Take(BigInteger hi)
+    {
+      Dafny.Sequence<T> _out11;
+      _out11 = Dafny._Companion_Sequence<T>.Take(this, hi);
+      return _out11;
+    }
+    public Dafny.Sequence<T> Subsequence(BigInteger lo, BigInteger hi)
+    {
+      Dafny.Sequence<T> _out12;
+      _out12 = Dafny._Companion_Sequence<T>.Subsequence(this, lo, hi);
+      return _out12;
+    }
+    public void __ctor(Dafny.ImmutableArray<T> @value)
+    {
+      (this)._value = @value;
+    }
+    public BigInteger Length() {
+      return ((this).@value).Length();
+    }
+    public Dafny.ImmutableArray<T> ToArray()
+    {
+      Dafny.ImmutableArray<T> ret = default(Dafny.ImmutableArray<T>);
+      ret = (this).@value;
+      return ret;
+      return ret;
+    }
+    public  Dafny.ImmutableArray<T> _value {get; set;}
+    public Dafny.ImmutableArray<T> @value { get {
+      return this._value;
+    } }
+  }
+
+  public partial class ConcatSequence<T> : Dafny.Sequence<T> {
+    public ConcatSequence() {
+      this._left = default(Dafny.Sequence<T>);
+      this._right = default(Dafny.Sequence<T>);
+      this._length = BigInteger.Zero;
+    }
+    public T Select(BigInteger index)
+    {
+      T _out13;
+      _out13 = Dafny._Companion_Sequence<T>.Select(this, index);
+      return _out13;
+    }
+    public Dafny.Sequence<T> Drop(BigInteger lo)
+    {
+      Dafny.Sequence<T> _out14;
+      _out14 = Dafny._Companion_Sequence<T>.Drop(this, lo);
+      return _out14;
+    }
+    public Dafny.Sequence<T> Take(BigInteger hi)
+    {
+      Dafny.Sequence<T> _out15;
+      _out15 = Dafny._Companion_Sequence<T>.Take(this, hi);
+      return _out15;
+    }
+    public Dafny.Sequence<T> Subsequence(BigInteger lo, BigInteger hi)
+    {
+      Dafny.Sequence<T> _out16;
+      _out16 = Dafny._Companion_Sequence<T>.Subsequence(this, lo, hi);
+      return _out16;
+    }
+    public void __ctor(Dafny.Sequence<T> left, Dafny.Sequence<T> right)
+    {
+      (this)._left = left;
+      (this)._right = right;
+      (this)._length = ((left).Length()) + ((right).Length());
+    }
+    public BigInteger Length() {
+      return (this).length;
+    }
+    public Dafny.ImmutableArray<T> ToArray()
+    {
+      Dafny.ImmutableArray<T> ret = default(Dafny.ImmutableArray<T>);
+      Dafny.Vector<T> _7_builder;
+      Dafny.Vector<T> _nw1 = new Dafny.Vector<T>();
+      _nw1.__ctor((this).length);
+      _7_builder = _nw1;
+      Dafny.Vector<Dafny.Sequence<T>> _8_stack;
+      Dafny.Vector<Dafny.Sequence<T>> _nw2 = new Dafny.Vector<Dafny.Sequence<T>>();
+      _nw2.__ctor(new BigInteger(10));
+      _8_stack = _nw2;
+      Dafny.__default.AppendOptimized<T>(_7_builder, this, _8_stack);
+      Dafny.ImmutableArray<T> _out17;
+      _out17 = (_7_builder).Freeze();
+      ret = _out17;
+      return ret;
+    }
+    public  Dafny.Sequence<T> _left {get; set;}
+    public Dafny.Sequence<T> left { get {
+      return this._left;
+    } }
+    public  Dafny.Sequence<T> _right {get; set;}
+    public Dafny.Sequence<T> right { get {
+      return this._right;
+    } }
+    public  BigInteger _length {get; set;}
+    public BigInteger length { get {
+      return this._length;
+    } }
+  }
+
+  public partial class LazySequence<T> : Dafny.Sequence<T> {
+    public LazySequence() {
+      this._length = BigInteger.Zero;
+      this._box = default(Dafny.AtomicBox<Dafny.Sequence<T>>);
+    }
+    public T Select(BigInteger index)
+    {
+      T _out18;
+      _out18 = Dafny._Companion_Sequence<T>.Select(this, index);
+      return _out18;
+    }
+    public Dafny.Sequence<T> Drop(BigInteger lo)
+    {
+      Dafny.Sequence<T> _out19;
+      _out19 = Dafny._Companion_Sequence<T>.Drop(this, lo);
+      return _out19;
+    }
+    public Dafny.Sequence<T> Take(BigInteger hi)
+    {
+      Dafny.Sequence<T> _out20;
+      _out20 = Dafny._Companion_Sequence<T>.Take(this, hi);
+      return _out20;
+    }
+    public Dafny.Sequence<T> Subsequence(BigInteger lo, BigInteger hi)
+    {
+      Dafny.Sequence<T> _out21;
+      _out21 = Dafny._Companion_Sequence<T>.Subsequence(this, lo, hi);
+      return _out21;
+    }
+    public void __ctor(Dafny.Sequence<T> wrapped)
+    {
+      Dafny.AtomicBox<Dafny.Sequence<T>> _9_box;
+      Dafny.AtomicBox<Dafny.Sequence<T>> _out22;
+      _out22 = Dafny.AtomicBox<Dafny.Sequence<T>>.Make(wrapped);
+      _9_box = _out22;
+      (this)._box = _9_box;
+      (this)._length = (wrapped).Length();
+    }
+    public BigInteger Length() {
+      return (this).length;
+    }
+    public Dafny.ImmutableArray<T> ToArray()
+    {
+      Dafny.ImmutableArray<T> ret = default(Dafny.ImmutableArray<T>);
+      Dafny.Sequence<T> _10_expr;
+      Dafny.Sequence<T> _out23;
+      _out23 = ((this).box).Get();
+      _10_expr = _out23;
+      Dafny.ImmutableArray<T> _out24;
+      _out24 = (_10_expr).ToArray();
+      ret = _out24;
+      Dafny.ArraySequence<T> _11_arraySeq;
+      Dafny.ArraySequence<T> _nw3 = new Dafny.ArraySequence<T>();
+      _nw3.__ctor(ret);
+      _11_arraySeq = _nw3;
+      ((this).box).Put(_11_arraySeq);
+      return ret;
+    }
+    public  BigInteger _length {get; set;}
+    public BigInteger length { get {
+      return this._length;
+    } }
+    public  Dafny.AtomicBox<Dafny.Sequence<T>> _box {get; set;}
+    public Dafny.AtomicBox<Dafny.Sequence<T>> box { get {
+      return this._box;
+    } }
+  }
+
+  public partial class __default {
+    public static Dafny.Sequence<__T> Concatenate<__T>(Dafny.Sequence<__T> left, Dafny.Sequence<__T> right)
+    {
+      Dafny.Sequence<__T> ret = default(Dafny.Sequence<__T>);
+      Dafny.ConcatSequence<__T> _12_c;
+      Dafny.ConcatSequence<__T> _nw4 = new Dafny.ConcatSequence<__T>();
+      _nw4.__ctor(left, right);
+      _12_c = _nw4;
+      Dafny.LazySequence<__T> _nw5 = new Dafny.LazySequence<__T>();
+      _nw5.__ctor(_12_c);
+      ret = _nw5;
+      return ret;
+    }
+    public static void AppendRecursive<__T>(Dafny.Vector<__T> builder, Dafny.Sequence<__T> e)
+    {
+      if (Dafny.Helpers.Let<Dafny.Sequence<__T>, bool>(e, _is_0 => _is_0 is Dafny.ConcatSequence<__T>)) {
+        Dafny.ConcatSequence<__T> _13_concat;
+        _13_concat = ((Dafny.ConcatSequence<__T>)(e));
+        Dafny.__default.AppendRecursive<__T>(builder, (_13_concat).left);
+        Dafny.__default.AppendRecursive<__T>(builder, (_13_concat).right);
+      } else if (Dafny.Helpers.Let<Dafny.Sequence<__T>, bool>(e, _is_1 => _is_1 is Dafny.LazySequence<__T>)) {
+        Dafny.LazySequence<__T> _14_lazy;
+        _14_lazy = ((Dafny.LazySequence<__T>)(e));
+        Dafny.Sequence<__T> _15_boxed;
+        Dafny.Sequence<__T> _out25;
+        _out25 = ((_14_lazy).box).Get();
+        _15_boxed = _out25;
+        Dafny.__default.AppendRecursive<__T>(builder, _15_boxed);
+      } else {
+        Dafny.ImmutableArray<__T> _16_a;
+        Dafny.ImmutableArray<__T> _out26;
+        _out26 = (e).ToArray();
+        _16_a = _out26;
+        (builder).Append(_16_a);
+      }
+    }
+    public static void AppendOptimized<__T>(Dafny.Vector<__T> builder, Dafny.Sequence<__T> e, Dafny.Vector<Dafny.Sequence<__T>> stack)
+    {
+    TAIL_CALL_START: ;
+      if (Dafny.Helpers.Let<Dafny.Sequence<__T>, bool>(e, _is_2 => _is_2 is Dafny.ConcatSequence<__T>)) {
+        Dafny.ConcatSequence<__T> _17_concat;
+        _17_concat = ((Dafny.ConcatSequence<__T>)(e));
+        (stack).AddLast((_17_concat).right);
+        Dafny.Vector<__T> _in0 = builder;
+        Dafny.Sequence<__T> _in1 = (_17_concat).left;
+        Dafny.Vector<Dafny.Sequence<__T>> _in2 = stack;
+        builder = _in0;
+        e = _in1;
+        stack = _in2;
+        goto TAIL_CALL_START;
+      } else if (Dafny.Helpers.Let<Dafny.Sequence<__T>, bool>(e, _is_3 => _is_3 is Dafny.LazySequence<__T>)) {
+        Dafny.LazySequence<__T> _18_lazy;
+        _18_lazy = ((Dafny.LazySequence<__T>)(e));
+        Dafny.Sequence<__T> _19_boxed;
+        Dafny.Sequence<__T> _out27;
+        _out27 = ((_18_lazy).box).Get();
+        _19_boxed = _out27;
+        Dafny.Vector<__T> _in3 = builder;
+        Dafny.Sequence<__T> _in4 = _19_boxed;
+        Dafny.Vector<Dafny.Sequence<__T>> _in5 = stack;
+        builder = _in3;
+        e = _in4;
+        stack = _in5;
+        goto TAIL_CALL_START;
+      } else if (Dafny.Helpers.Let<Dafny.Sequence<__T>, bool>(e, _is_4 => _is_4 is Dafny.ArraySequence<__T>)) {
+        Dafny.ArraySequence<__T> _20_a;
+        _20_a = ((Dafny.ArraySequence<__T>)(e));
+        (builder).Append((_20_a).@value);
+        if ((stack.size).Sign == 1) {
+          Dafny.Sequence<__T> _21_next;
+          Dafny.Sequence<__T> _out28;
+          _out28 = (stack).RemoveLast();
+          _21_next = _out28;
+          Dafny.Vector<__T> _in6 = builder;
+          Dafny.Sequence<__T> _in7 = _21_next;
+          Dafny.Vector<Dafny.Sequence<__T>> _in8 = stack;
+          builder = _in6;
+          e = _in7;
+          stack = _in8;
+          goto TAIL_CALL_START;
+        }
+      } else {
+      }
+    }
+  }
+} // end of namespace Dafny
 namespace _module {
 
 } // end of namespace _module
